src/SerialFacts.v
@@ -2,6 +2,8 @@ Require Import Bool List String Peano_dec.
 Require Import Common ListSupport FMap.
 Require Import Syntax Semantics SemFacts StepDet Serial.
 
+Require Import Omega.
+
 Set Implicit Arguments.
 
 Lemma SubHistory_refl:
@@ -60,23 +62,64 @@ Proof.
     unfold isExternal in *.
     rewrite H1 in H; assumption.
   - constructor; auto.
-    unfold isInternal in *.
-    rewrite H2 in H1; assumption.
+    + unfold isInternal in *.
+      rewrite H4 in H1; assumption.
+    + unfold isInternal in *.
+      rewrite H4 in H2; assumption.
   - constructor; auto.
-    unfold isExternal in *.
-    rewrite H1 in H0; assumption.
+    + unfold isInternal in *.
+      rewrite H2 in H0; assumption.
+    + unfold isExternal in *.
+      rewrite H2 in H1; assumption.
 Qed.
 
-Lemma atomic_rs_out:
+Lemma atomic_rs_out_1:
   forall sys rqin hdl rsout hst mouts orsout,
     Atomic sys rqin (IlblOuts (Some hdl) (rsout :: nil) :: hst) mouts orsout ->
     isExternal sys (mid_to (msg_id (tmsg_msg rsout))) = true ->
     mouts = nil /\ orsout = Some rsout.
 Proof.
   intros; inv H.
-  - exfalso; inv H9.
-    eapply internal_external_false; eauto.
+  - exfalso; inv H10.
+    eapply (internal_external_false _ _ H2 H0); eauto.
   - auto.
+Qed.
+
+Lemma atomic_rs_out_2:
+  forall sys rqin hst mouts rsout,
+    Atomic sys rqin hst mouts (Some rsout) ->
+    hst <> nil /\
+    isExternal sys (mid_to (msg_id (tmsg_msg rsout))) = true /\
+    mouts = nil /\
+    exists hdl hst', hst = (IlblOuts (Some hdl) (rsout :: nil) :: hst').
+Proof.
+  intros; inv H.
+  repeat split; eauto.
+  discriminate.
+Qed.
+
+Lemma atomic_mouts_tinfo:
+  forall sys rqin hst mouts orsout,
+    Atomic sys rqin hst mouts orsout ->
+    forall st1 st2,
+      steps_det sys st1 hst st2 ->
+      ForallMP (fun tmsg => tmsg_info tmsg = Some rqin) mouts.
+Proof.
+  induction 1; simpl; intros.
+  - constructor; auto.
+  - inv H4; apply ForallMP_distributeMsgs.
+    + eapply ForallMP_deqMP; eauto.
+    + inv H10.
+      remember (match tmsg_info fmsg with
+                | Some finfo => finfo
+                | None => {| tinfo_tid := nts; tinfo_rqin := tmsg_msg fmsg |}
+                end) as ntinfo; clear Heqntinfo.
+      specialize (IHAtomic _ _ H8).
+      eapply ForallMP_forall in IHAtomic; eauto.
+      simpl in IHAtomic; inv IHAtomic.
+      clear; induction (rule_outs _ _ _); [constructor|].
+      constructor; auto.
+  - constructor.
 Qed.
 
 Lemma trsMessages_app:
@@ -87,26 +130,442 @@ Proof.
   intros; apply filter_app.
 Qed.
 
+Lemma trsMessages_In:
+  forall tmsg ti mp,
+    In tmsg mp ->
+    tmsg_info tmsg = Some ti ->
+    In tmsg (trsMessages ti mp).
+Proof.
+  induction mp; simpl; intros; auto.
+  destruct H; subst.
+  - rewrite H0.
+    destruct (tinfo_dec ti ti); [|elim n; reflexivity].
+    left; reflexivity.
+  - find_if_inside; auto.
+    right; auto.
+Qed.
+
+Lemma trsMessages_In_tinfo:
+  forall tmsg ti mp,
+    In tmsg (trsMessages ti mp) ->
+    tmsg_info tmsg = Some ti.
+Proof.
+  induction mp; simpl; intros; [elim H|].
+  remember (tmsg_info a) as oti; destruct oti as [ati|]; auto.
+  destruct (tinfo_dec ati ti); subst; auto.
+  inv H; auto.
+Qed.
+  
+Lemma trsMessages_SubList:
+  forall ti mp1 mp2,
+    SubList mp1 mp2 ->
+    SubList (trsMessages ti mp1) (trsMessages ti mp2).
+Proof.
+  induction mp1; simpl; intros; [apply SubList_nil|].
+  apply SubList_cons_inv in H; dest.
+  remember (tmsg_info a) as tinfo; destruct tinfo; auto.
+  destruct (tinfo_dec t ti); subst; auto.
+  apply SubList_cons; auto.
+  apply trsMessages_In; auto.
+Qed.
+
+Lemma trsMessages_deqMP_SubList:
+  forall ti from to chn mp,
+    SubList (trsMessages ti (deqMP from to chn mp))
+            (trsMessages ti mp).
+Proof.
+  intros.
+  apply trsMessages_SubList.
+  apply deqMP_SubList.
+Qed.
+
+Lemma trsMessages_toTMsg:
+  forall ti msgs,
+    trsMessages ti (toTMsgs ti msgs) = toTMsgs ti msgs.
+Proof.
+  induction msgs; simpl; intros; [reflexivity|].
+  destruct (tinfo_dec ti ti); [|elim n; reflexivity].
+  rewrite IHmsgs; reflexivity.
+Qed.
+
+Lemma trsMessages_deqMP_comm:
+  forall rqin from to chn mp tmsg,
+    firstMP from to chn mp = Some tmsg ->
+    tmsg_info tmsg = Some rqin ->
+    trsMessages rqin (deqMP from to chn mp) =
+    deqMP from to chn (trsMessages rqin mp).
+Proof.
+  induction mp; simpl; intros; [reflexivity|].
+  unfold firstMP in H; simpl in H.
+  destruct (msgAddr_dec _ _).
+  - inv H; rewrite H0.
+    destruct (tinfo_dec _ _); [|elim n; reflexivity].
+    simpl; destruct (msgAddr_dec _ _); [|elim n; assumption].
+    reflexivity.
+  - specialize (IHmp _ H H0).
+    simpl; destruct (tmsg_info a); [|assumption].
+    destruct (tinfo_dec _ _); subst; [|assumption].
+    simpl; destruct (msgAddr_dec _ _); [elim n; assumption|].
+    rewrite IHmp; reflexivity.
+Qed.
+
+Lemma msgs_tinfo_old':
+  forall sys sti ll st,
+    steps_det sys sti ll st ->
+    sti = getStateInit sys ->
+    ForallMP (fun tmsg =>
+                match tmsg_info tmsg with
+                | Some tinfo => tinfo_tid tinfo <= tst_tid st
+                | None => True
+                end) (tst_msgs st).
+Proof.
+  induction 1; simpl; intros; subst.
+  - cbn; constructor.
+  - specialize (IHsteps eq_refl).
+    inv H0; simpl.
+    + apply IHsteps; auto.
+    + apply ForallMP_enqMP; auto.
+      subst; cbn; auto.
+    + simpl in IHsteps.
+      apply ForallMP_distributeMsgs.
+      * destruct (tmsg_info fmsg) as [tinfo|].
+        { apply ForallMP_deqMP; auto. }
+        { apply ForallMP_deqMP.
+          apply ForallMP_forall; intros.
+          eapply ForallMP_forall in IHsteps; eauto.
+          destruct (tmsg_info msg); [omega|auto].
+        }
+      * apply firstMP_inMP in H5.
+        eapply ForallMP_forall in IHsteps; eauto.
+        destruct (tmsg_info fmsg) as [ftinfo|].
+        { clear -IHsteps Hts.
+          induction (rule_outs _ _ _); [constructor|].
+          simpl; find_if_inside; auto.
+          constructor; auto.
+        }
+        { clear.
+          induction (rule_outs _ _ _); [constructor|].
+          simpl; find_if_inside; auto.
+          constructor; auto.
+          simpl; omega.
+        }
+Qed.
+
+Lemma msgs_tinfo_old:
+  forall sys st,
+    Reachable steps_det sys st ->
+    ForallMP (fun tmsg =>
+                match tmsg_info tmsg with
+                | Some tinfo => tinfo_tid tinfo <= tst_tid st
+                | None => True
+                end) (tst_msgs st).
+Proof.
+  intros; inv H.
+  eapply msgs_tinfo_old'; eauto.
+Qed.
+
+Lemma external_msg_in_tinfo':
+  forall sys sti ll st,
+    steps_det sys sti ll st ->
+    sti = getStateInit sys ->
+    forall msgs,
+      msgs = tst_msgs st ->
+      forall tmsg,
+        InMP tmsg msgs ->
+        isExternal sys (mid_from (msg_id (tmsg_msg tmsg))) = true ->
+        tmsg_info tmsg = None.
+Proof.
+  induction 1; simpl; intros; subst; [inv H1|].
+  specialize (IHsteps eq_refl _ eq_refl).
+  inv H0; [eauto| |].
+
+  - simpl in H3.
+    apply inMP_enqMP_or in H3; destruct H3.
+    + subst; reflexivity.
+    + eapply IHsteps; eauto.
+
+  - simpl in H3.
+    apply inMP_distributeMsgs_or in H3; destruct H3.
+    + exfalso.
+      unfold intOuts in H0; apply filter_In in H0; destruct H0.
+      apply obj_in_sys_idx_internal in H1.
+      destruct H13.
+      clear -H0 H1 H3 H4.
+      induction (rule_outs _ _ _); [inv H0|].
+      inv H3; dest.
+      inv H0.
+      * simpl in H, H4.
+        unfold id in H; rewrite H in H4.
+        eapply internal_external_false; eauto.
+      * eapply IHl; eauto.
+    + eapply IHsteps; eauto.
+      simpl.
+      eapply inMP_deqMP; eauto.
+Qed.
+
+Lemma external_msg_in_tinfo:
+  forall sys st,
+    Reachable steps_det sys st ->
+    forall from to chn tmsg msgs,
+      msgs = tst_msgs st ->
+      firstMP from to chn msgs = Some tmsg ->
+      isExternal sys (mid_from (msg_id (tmsg_msg tmsg))) = true ->
+      tmsg_info tmsg = None.
+Proof.
+  intros; inv H.
+  eapply external_msg_in_tinfo'; eauto.
+  eapply firstMP_inMP; eauto.
+Qed.
+
+Lemma internal_msg_in_tinfo':
+  forall sys sti ll st,
+    steps_det sys sti ll st ->
+    sti = getStateInit sys ->
+    forall msgs,
+      msgs = tst_msgs st ->
+      forall tmsg,
+        InMP tmsg msgs ->
+        isInternal sys (mid_from (msg_id (tmsg_msg tmsg))) = true ->
+        exists tinfo, tmsg_info tmsg = Some tinfo.
+Proof.
+  induction 1; simpl; intros; subst; [inv H1|].
+  specialize (IHsteps eq_refl _ eq_refl).
+  inv H0; [eauto| |].
+
+  - simpl in H3.
+    apply inMP_enqMP_or in H3; destruct H3.
+    + exfalso; subst; simpl in *.
+      eauto using internal_external_false.
+    + eapply IHsteps; eauto.
+
+  - simpl in H3.
+    apply inMP_distributeMsgs_or in H3; destruct H3.
+    + clear -H0.
+      unfold intOuts in H0; apply filter_In in H0; destruct H0.
+      induction (rule_outs _ _ _); [inv H|].
+      inv H; auto.
+      simpl; eexists; reflexivity.
+    + eapply IHsteps; eauto.
+      simpl.
+      eapply inMP_deqMP; eauto.
+Qed.
+
+Lemma internal_msg_in_tinfo:
+  forall sys st,
+    Reachable steps_det sys st ->
+    forall from to chn tmsg msgs,
+      msgs = tst_msgs st ->
+      firstMP from to chn msgs = Some tmsg ->
+      isInternal sys (mid_from (msg_id (tmsg_msg tmsg))) = true ->
+      exists tinfo, tmsg_info tmsg = Some tinfo.
+Proof.
+  intros; inv H.
+  eapply internal_msg_in_tinfo'; eauto.
+  eapply firstMP_inMP; eauto.
+Qed.
+
+Lemma ts_monotone:
+  forall sys st1 lbl st2,
+    step_det sys st1 lbl st2 ->
+    tst_tid st1 <= tst_tid st2.
+Proof.
+  intros; inv H; auto.
+  simpl; destruct (tmsg_info fmsg); omega.
+Qed.
+
+Lemma reachable_hst_old':
+  forall sys hst sti st,
+    steps_det sys sti hst st ->
+    sti = getStateInit sys ->
+    Forall (fun tlbl =>
+              match tlbl with
+              | IlblOuts (Some hdl) _ =>
+                match tmsg_info hdl with
+                | Some tinfo => tinfo_tid tinfo <= tst_tid st
+                | None => True
+                end
+              | _ => True
+              end) hst.
+Proof.
+  induction 1; simpl; intros; subst; [constructor|].
+  constructor.
+  - assert (Reachable steps_det sys st2) by (econstructor; eauto).
+    apply msgs_tinfo_old in H1.
+    inv H0; simpl; auto.
+    simpl in H1.
+    apply firstMP_inMP in H6.
+    eapply ForallMP_forall in H1; eauto.
+    destruct (tmsg_info fmsg); auto.
+  - apply ts_monotone in H0.
+    specialize (IHsteps eq_refl).
+    clear -H0 IHsteps.
+    induction ll; simpl; intros; [constructor|].
+    inv IHsteps.
+    constructor; auto.
+    destruct a; auto.
+    destruct mhdl; auto.
+    destruct (tmsg_info t); auto.
+    omega.
+Qed.
+
+Lemma reachable_hst_old:
+  forall sys st1,
+    Reachable steps_det sys st1 ->
+    forall hst st2,
+      steps_det sys st1 hst st2 ->
+      Forall (fun tlbl =>
+                match tlbl with
+                | IlblOuts (Some hdl) _ =>
+                  match tmsg_info hdl with
+                  | Some tinfo => tinfo_tid tinfo <= tst_tid st2
+                  | None => True
+                  end
+                | _ => True
+                end) hst.
+Proof.
+  intros; inv H.
+  assert (steps_det sys (getStateInit sys) (hst ++ ll) st2).
+  { eapply steps_append; eauto. }
+  apply reachable_hst_old' in H; auto.
+  apply Forall_app_inv in H.
+  dest; auto.
+Qed.
+
 Lemma atomic_outs:
   forall sys rqin hst mouts orsout,
     Atomic sys rqin hst mouts orsout ->
     hst <> nil ->
-    forall st1 st2,
-      steps_det sys st1 hst st2 ->
-      trsMessages rqin (tst_msgs st2) = mouts.
+    forall st1,
+      Reachable steps_det sys st1 ->
+      forall st2,
+        steps_det sys st1 hst st2 ->
+        trsMessages rqin (tst_msgs st2) = mouts.
 Proof.
   induction 1; simpl; intros; [intuition idtac| |].
-  - inv H3.
-    inv H9; simpl in *.
+  - inv H6.
+    pose proof (atomic_mouts_tinfo H H10) as Htinfo.
+    eapply ForallMP_forall in Htinfo; eauto.
+    inv H12; simpl in *.
     unfold distributeMsgs.
     rewrite trsMessages_app.
+    destruct hst as [|lbl hst].
 
-    (* Hint: case analysis on [hst]:
-     * - nil: invert H
-     * - cons: use IHAtomic
-     *)
-    
-Admitted.
+    + inv H10.
+      clear IHAtomic; inv H.
+      unfold InMP in H0; Common.dest_in.
+      unfold toTMsg in H; cbn in H; inv H.
+      eapply external_msg_in_tinfo in H14; eauto.
+      rewrite H14 in *; clear H14.
+      inv H9.
+      f_equal.
+      
+      * pose proof (msgs_tinfo_old H5); simpl in H.
+        replace (deqMP from to chn
+                       (enqMP (toTMsg {| tinfo_tid := nts; tinfo_rqin := tmsg_msg fmsg |}
+                                      (tmsg_msg fmsg)) nil))
+          with (nil (A:= TMsg)).
+        { (* NOTE: better to extract lemmas? *)
+          clear -H Hts.
+          assert (trsMessages {| tinfo_tid := nts; tinfo_rqin := tmsg_msg fmsg |} oims = nil).
+          { induction oims; [reflexivity|].
+            inv H; simpl.
+            destruct (tmsg_info a); auto.
+            destruct (tinfo_dec _ _); auto.
+            subst; simpl in H2; omega.
+          }
+          pose proof (trsMessages_deqMP_SubList
+                        {| tinfo_tid := nts; tinfo_rqin := tmsg_msg fmsg |}
+                        fidx (obj_idx obj) fchn oims).
+          rewrite H0 in H1.
+          apply SubList_nil_inv in H1; auto.
+        }
+        { unfold deqMP, enqMP; simpl.
+          apply firstMP_ValidMsgId in H3.
+          rewrite <-H3; simpl.
+          destruct (msgAddr_dec _ _); [|elim n; reflexivity].
+          reflexivity.
+        }
+          
+      * replace (intOuts sys (toTMsgs {| tinfo_tid := nts; tinfo_rqin := tmsg_msg fmsg |}
+                                      (rule_outs frule os (msg_value (tmsg_msg fmsg)))))
+          with (toTMsgs {| tinfo_tid := nts; tinfo_rqin := tmsg_msg fmsg |}
+                        (rule_outs frule os (msg_value (tmsg_msg fmsg)))).
+        { apply trsMessages_toTMsg. }
+        { clear -H2.
+          induction (toTMsgs {| tinfo_tid := nts; tinfo_rqin := tmsg_msg fmsg |}
+                             (rule_outs frule os (msg_value (tmsg_msg fmsg))));
+            [reflexivity|].
+          inv H2; simpl; dest.
+          rewrite H1.
+          rewrite IHl at 1 by assumption; reflexivity.
+        }
+
+    + assert (exists tinfo, tmsg_info fmsg = Some tinfo).
+      { inv H5.
+        eapply internal_msg_in_tinfo; [| |eassumption|eassumption].
+        { econstructor; eapply steps_append; eauto. }
+        { reflexivity. }
+      }
+      destruct H6 as [tinfo ?]; rewrite H6 in *.
+      inv Htinfo.
+      assert (lbl :: hst <> nil) by discriminate.
+      specialize (IHAtomic H7 _ H5 _ H10); clear H7; subst.
+      apply trsMessages_In_tinfo in H0; inv H0.
+      f_equal.
+      * assert (from = fidx /\ to = obj_idx obj /\ chn = fchn).
+        { apply firstMP_ValidMsgId in H3; apply firstMP_ValidMsgId in H14.
+          unfold ValidMsgId in *; simpl in *.
+          rewrite H3 in H14; inv H14; auto.
+        }
+        dest; subst; simpl.
+        eapply trsMessages_deqMP_comm; eauto.
+      * rewrite intOuts_Forall by assumption.
+        apply trsMessages_toTMsg.
+
+  - inv H4.
+    pose proof (atomic_mouts_tinfo H H8) as Htinfo.
+    eapply ForallMP_forall in Htinfo; [|left; reflexivity].
+    inv H; [exfalso; eapply internal_external_false; eauto|].
+    assert (IlblOuts (Some hdl0) houts :: hst0 <> nil) by discriminate.
+    specialize (IHAtomic H _ H3 _ H8).
+    clear H H2.
+    inv H10; simpl in *.
+
+    assert (exists tinfo, tmsg_info fmsg = Some tinfo).
+    { inv H3.
+      eapply internal_msg_in_tinfo; [| |eassumption|eassumption].
+      { econstructor; eapply steps_append; eauto. }
+      { reflexivity. }
+    }
+    destruct H as [tinfo ?]; rewrite H in *.
+    inv Htinfo.
+
+    rewrite H2.
+    replace (intOuts sys (rsout :: nil)) with (nil (A:= TMsg))
+      by (simpl; rewrite external_not_internal by assumption; reflexivity).
+    unfold distributeMsgs; rewrite app_nil_r.
+
+    rewrite trsMessages_deqMP_comm with (tmsg:= fmsg); try assumption.
+    rewrite IHAtomic.
+    simpl.
+    apply firstMP_ValidMsgId in H16. inv H16.
+    destruct (msgAddr_dec _ _); [|elim n; reflexivity].
+    reflexivity.
+Qed.
+
+Corollary atomic_rs_out_trsMessages_nil:
+  forall sys rqin hst mouts rsout,
+    Atomic sys rqin hst mouts (Some rsout) ->
+    forall st1,
+      Reachable steps_det sys st1 ->
+      forall st2,
+        steps_det sys st1 hst st2 ->
+        trsMessages rqin (tst_msgs st2) = nil.
+Proof.
+  intros.
+  pose proof (atomic_rs_out_2 H); dest; subst.
+  eapply atomic_outs; eauto.
+Qed.
 
 Theorem serializable_seqSteps_refines:
   forall sys,
